Work around postcondition issues

ulib/FStar.Pointer.Derived2.fst
@@ -24,7 +24,6 @@ let copy_buffer_contents_inv
   buffer_as_seq h' (gsub_buffer b idx_b len') == buffer_as_seq h (gsub_buffer a idx_a len')
 
 private
-assume
 val copy_buffer_contents_init
   (#t: typ)
   (a: buffer t) (* source *)
@@ -37,10 +36,9 @@ val copy_buffer_contents_init
   (requires (copy_buffer_contents_precond a idx_a b idx_b len h))
   (ensures (copy_buffer_contents_inv a idx_a b idx_b len 0ul h h))
 
-(*
-= buffer_readable_intro_empty h (gsub_buffer b idx_b 0ul);
+let copy_buffer_contents_init #t a idx_a b idx_b len h =
+  buffer_readable_intro_empty h (gsub_buffer b idx_b 0ul);
   Seq.lemma_eq_intro (buffer_as_seq h (gsub_buffer b idx_b 0ul)) (buffer_as_seq h (gsub_buffer a idx_a 0ul))
-*)
 
 private
 assume
@@ -65,7 +63,6 @@ val copy_buffer_contents_advance
   ))
 
 private
-assume
 val copy_buffer_contents_aux
   (#t: typ)
   (a: buffer t) (* source *)
@@ -76,16 +73,15 @@ val copy_buffer_contents_aux
   (len': UInt32.t)
   (h: Ghost.erased HS.mem)
 : HST.Stack unit
-  (requires (fun h0 ->
+  (requires (fun h0 -> 
     copy_buffer_contents_inv a idx_a b idx_b len len' (Ghost.reveal h) h0
   ))
   (ensures (fun h0 _ h1 ->
     copy_buffer_contents_inv a idx_a b idx_b len len' (Ghost.reveal h) h0 /\
     copy_buffer_contents_postcond a idx_a b idx_b len (Ghost.reveal h) h1
   ))
-//  (decreases (UInt32.v len - UInt32.v len'))
+  (decreases (UInt32.v len - UInt32.v len'))
 
-(*
 let rec copy_buffer_contents_aux #t a idx_a b idx_b len len' h =
   if len = len'
   then ()
@@ -93,10 +89,26 @@ let rec copy_buffer_contents_aux #t a idx_a b idx_b len len' h =
     copy_buffer_contents_advance a idx_a b idx_b len len' h;
     copy_buffer_contents_aux a idx_a b idx_b len (UInt32.add len' 1ul) h
   end
-*)
 
-let copy_buffer_contents #t a idx_a b idx_b len =
-  let h0 = HST.get () in
+(* FIXME: Does not work if I directly try to define copy_buffer_contents *)
+
+let copy_buffer_contents'
+  (#t: typ)
+  (a: buffer t) (* source *)
+  (idx_a: UInt32.t)
+  (b: buffer t) (* destination *)
+  (idx_b: UInt32.t)
+  (len: UInt32.t)
+: HST.Stack unit
+  (requires (fun h ->
+    copy_buffer_contents_precond a idx_a b idx_b len h
+//    copy_buffer_contents_inv a idx_a b idx_b len 0ul h h
+  ))
+  (ensures (fun h0 _ h1 ->
+    copy_buffer_contents_postcond a idx_a b idx_b len h0 h1
+  ))
+= let h0 = HST.get () in
   copy_buffer_contents_init a idx_a b idx_b len h0;
-  copy_buffer_contents_aux a idx_a b idx_b len 0ul (Ghost.hide h0);
-  admit ()
+  copy_buffer_contents_aux a idx_a b idx_b len 0ul (Ghost.hide h0)
+
+let copy_buffer_contents = copy_buffer_contents'
